Run the block verifier in the HeapSpec monad

case_study/RiscvPmp/BlockVer/Verifier.v
@@ -27,6 +27,7 @@
 (******************************************************************************)
 
 From Coq Require Import
+     Classes.Morphisms_Prop
      ZArith.ZArith
      Lists.List
      micromega.Lia
@@ -39,6 +40,7 @@ From Katamaran Require Import
      Notations
      Semantics
      Bitvector
+     Refinement.Monads
      Sep.Hoare
      Shallow.Executor
      Shallow.Soundness
@@ -71,796 +73,734 @@ Open Scope string_scope.
 Open Scope ctx_scope.
 Open Scope Z_scope.
 
+Import RiscvPmpIrisBase RiscvPmpIrisInstance.
+#[local] Notation "a '↦' t" := (reg_pointsTo a t) (at level 70).
+#[local] Notation "a '↦ₘ' t" := (interp_ptsto a t) (at level 70).
+
 Module ns := stdpp.namespaces.
 
 (*   Definition pmp_entry_cfg := ty_prod ty_pmpcfg_ent ty_xlenbits. *)
 
-Module BlockVerificationDerived2.
+Section BlockVerificationDerived.
 
-  Import RiscvPmpBlockVerifSpec.
   Import RiscvPmpBlockVerifExecutor.
-  Import Symbolic.
-
-  Import ModalNotations.
-
-  Definition M : TYPE -> TYPE := SStoreSpec [] [].
-
-  Definition pure {A} : ⊢ A -> M A := SStoreSpec.pure.
-  Definition bind {A B} : ⊢ M A -> □(A -> M B) -> M B := SStoreSpec.bind.
-  Definition angelic : ⊢ ∀ σ : Ty, M (STerm σ) := @SStoreSpec.angelic [] None.
-  Definition demonic : ⊢ ∀ σ : Ty, M (STerm σ) := @SStoreSpec.demonic [] None.
-  Definition assert : ⊢ Formula -> M Unit := SStoreSpec.assert_formula.
-  Definition assume : ⊢ Formula -> M Unit := SStoreSpec.assume_formula.
-
-  Definition produce_chunk : ⊢ Chunk -> M Unit := SStoreSpec.produce_chunk.
-  Definition consume_chunk : ⊢ Chunk -> M Unit := SStoreSpec.consume_chunk.
-
-  Definition produce {Σ} (asn : Assertion Σ) : ⊢ Sub Σ -> M Unit := SStoreSpec.produce asn.
-  Definition consume {Σ} (asn : Assertion Σ) : ⊢ Sub Σ -> M Unit := SStoreSpec.consume asn.
-
-  Notation "ω ∣ x <- ma ;; mb" :=
-    (bind ma (fun _ ω x => mb))
-      (at level 80, x at next level,
-        ma at next level, mb at level 200,
-        right associativity).
-
-  Definition exec_instruction_any (i : AST) : ⊢ STerm ty_xlenbits -> M (STerm ty_xlenbits) :=
-    let inline_fuel := 10%nat in
-    fun _ a =>
-      ω2 ∣ _ <- produce_chunk (chunk_ptsreg pc a) ;;
-      ω4 ∣ _ <- produce_chunk (chunk_user ptstoinstr [persist__term a ω2; term_val ty_ast i]) ;;
-      ω6 ∣ an <- @demonic _ _ ;;
-      ω7 ∣ _ <- produce_chunk (chunk_ptsreg nextpc an) ;;
-      ω8 ∣ _ <- SStoreSpec.exec default_config inline_fuel (FunDef step) ;;
-      ω9 ∣ _ <- consume_chunk (chunk_user ptstoinstr [persist__term a (ω2 ∘ ω4 ∘ ω6 ∘ ω7 ∘ ω8); term_val ty_ast i]) ;;
-      ω10 ∣ na <- @angelic _ _ ;;
-      ω11 ∣ _ <- consume_chunk (chunk_ptsreg nextpc na) ;;
-      ω12 ∣ _ <- consume_chunk (chunk_ptsreg pc (persist__term na ω11)) ;;
-      pure (persist__term na (ω11 ∘ ω12)).
-
-  Definition exec_instruction (i : AST) : ⊢ M Unit :=
-    let inline_fuel := 10%nat in
-    fun _ =>
-      ω1 ∣ a <- @demonic _ _ ;;
-      ω2 ∣ na <- exec_instruction_any i a ;;
-      assert (formula_relop bop.eq na (term_binop bop.bvadd (persist__term a ω2) (term_val ty_word bv_instrsize))).
-
-
-  Fixpoint exec_block_addr (b : list AST) : ⊢ STerm ty_xlenbits -> STerm ty_xlenbits -> M (STerm ty_xlenbits) :=
-    fun _ ainstr apc =>
-      match b with
-      | nil       => pure apc
-      | cons i b' =>
-        ω1 ∣ _ <- assert (formula_relop bop.eq ainstr apc) ;;
-        ω2 ∣ apc' <- exec_instruction_any i (persist__term apc ω1) ;;
-        @exec_block_addr b' _ (term_binop bop.bvadd (persist__term ainstr (ω1 ∘ ω2)) (term_val ty_word bv_instrsize)) apc'
-      end.
-
-  (* Definition exec_double_addr {Σ : World} *)
-  (*   (req : Assertion (Σ ▻ ("a":: ty_xlenbits))) (b : list AST) : M (STerm ty_xlenbits) Σ := *)
-  (*   ω1 ∣ an <- @demonic _ _ ;; *)
-  (*   ω2 ∣ _ <- produce (w := wsnoc _ _) req (acc_snoc_left ω1 _ an);; *)
-  (*   @exec_block_addr b _ (persist__term an ω2) (persist__term an ω2). *)
-
-  Definition exec_triple_addr {Σ : World}
-    (req : Assertion (Σ ▻ ("a"::ty_xlenbits))) (b : list AST)
-    (ens : Assertion (Σ ▻ ("a"::ty_xlenbits) ▻ ("an"::ty_xlenbits))) : M Unit Σ :=
-    ω1 ∣ a <- @demonic _ _ ;;
-    ω2 ∣ _ <- produce  req (sub_snoc (sub_acc ω1) _ a) ;;
-    ω3 ∣ na <- @exec_block_addr b _ (persist__term a ω2) (persist__term a ω2) ;;
-    consume ens
-      (sub_snoc (sub_snoc (sub_acc (ω1 ∘ ω2 ∘ ω3)) ("a"∷ty_xlenbits) (persist__term a (ω2 ∘ ω3)))
-         ("an"∷ty_xlenbits) na).
-
-  (* This is a VC for triples, for doubles we probably need to talk
-     about the continuation of a block. *)
-  Definition VC__addr {Σ : LCtx} (req : Assertion {| wctx := Σ ▻ ("a":: ty_xlenbits); wco := []%ctx |}) (b : list AST)
-    (ens : Assertion {| wctx := Σ ▻ ("a"::ty_xlenbits) ▻ ("an"::ty_xlenbits); wco := []%ctx |}) : 𝕊 ε :=
-    SymProp.demonic_close
-      (@exec_triple_addr
-         {| wctx := Σ; wco := []%ctx |}
-         req b ens
-         (* Could include leakcheck here *)
-         (fun _ _ _ _ h => SymProp.block)
-         []%env []%list).
+  Import RiscvPmpBlockVerifShalExecutor.
 
   Definition safeE {Σ} : 𝕊 Σ -> Prop :=
     fun P => VerificationConditionWithErasure (Erasure.erase_symprop P).
 
-  Lemma safeE_safe (p : 𝕊 wnil) (ι : Valuation wnil) : safeE p -> SymProp.safe p [].
-  Proof. apply verification_condition_with_erasure_sound. Qed.
-
-End BlockVerificationDerived2.
-
-Module BlockVerification3.
-
-  Import RiscvPmpBlockVerifSpec.
-  Import RiscvPmpBlockVerifExecutor.
-  Import Symbolic.
-
-  Import ModalNotations.
-  Import BlockVerificationDerived2.
-
-  Inductive AnnotInstr :=
-  | AnnotAST : forall (i : AST), AnnotInstr
-  | AnnotDebugBreak : AnnotInstr
-  | AnnotLemmaInvocation : forall {Δ} (l : 𝑳 Δ) (es : NamedEnv (Exp [ctx]) Δ), AnnotInstr
-  .
-
-  Record DebugBlockver (Σ : LCtx) : Type :=
-    MkDebugBlockver {
-        debug_blockver_pathcondition          : PathCondition Σ;
-        debug_blockver_heap                   : SHeap Σ;
-      }.
-  #[export] Instance SubstDebugBlockver : Subst DebugBlockver :=
-    fun Σ0 d Σ1 ζ01 =>
-      match d with
-      | MkDebugBlockver pc1 h => MkDebugBlockver (subst pc1 ζ01) (subst h ζ01)
-      end.
-
-  #[export] Instance SubstLawsDebugBlockver : SubstLaws DebugBlockver.
+  Definition safeE_safe (p : 𝕊 wnil) (ι : Valuation wnil) : safeE p -> SymProp.safe p [].
   Proof.
-    constructor.
-    - intros ? []; cbn; now rewrite ?subst_sub_id.
-    - intros ? ? ? ? ? []; cbn; now rewrite ?subst_sub_comp.
+    unfold safeE.
+    destruct 1 as [H].
+    now apply Erasure.erase_safe'.
   Qed.
 
-  Import option.notations.
-  #[export] Instance OccursCheckDebugBlockver : OccursCheck DebugBlockver :=
-    fun Σ x xIn d =>
-      match d with
-      | MkDebugBlockver pc1 h =>
-          pc' <- occurs_check xIn pc1 ;;
-          h'  <- occurs_check xIn h ;;
-          Some (MkDebugBlockver pc' h')
-      end.
+  Section Symbolic.
 
+    Import ModalNotations.
+    Import SStoreSpec (evalStoreSpec, exec).
+    Import SHeapSpec SHeapSpec.notations.
+    Import asn.notations.
 
-  Fixpoint exec_block_addr (b : list AnnotInstr) : ⊢ STerm ty_xlenbits -> STerm ty_xlenbits -> M (STerm ty_xlenbits) :=
-    fun w0 ainstr apc =>
-      match b with
-      | nil       => pure apc
-      | cons instr b' =>
-          match instr with
-          | AnnotAST i => ω1 ∣ _ <- assert (formula_relop bop.eq ainstr apc) ;;
-                         ω2 ∣ apc' <- exec_instruction_any i (persist__term apc ω1) ;;
-                         @exec_block_addr b' _ (term_binop bop.bvadd (persist__term ainstr (ω1 ∘ ω2)) (term_val ty_word bv_instrsize)) apc'
-          | AnnotDebugBreak => SStoreSpec.debug
-                                (fun (δ0 : SStore [ctx] w0) (h0 : SHeap w0) =>
-                                   amsg.mk
-                                     {| debug_blockver_pathcondition := wco w0;
-                                       debug_blockver_heap := h0
-                                     |})
-                                (SStoreSpec.pure apc)
-          | AnnotLemmaInvocation l es =>
-              ω1 ∣ args <- SStoreSpec.eval_exps es (w:=w0) ;;
-              ω2 ∣ _ <- SStoreSpec.call_lemma (LEnv l) args ;;
-              @exec_block_addr b' _ (persist__term ainstr (ω1 ∘ ω2)) (persist__term apc (ω1 ∘ ω2))
-          end
-      end.
+    Definition exec_instruction_prologue (i : AST) :
+      Assertion ([ctx] ▻ ("a":: ty_xlenbits)) :=
+      pc     ↦ term_var "a" ∗
+      asn.chunk (chunk_user ptstoinstr [term_var "a"; term_val ty_ast i]) ∗
+      asn.exist "an" ty_xlenbits (nextpc ↦ term_var "an").
 
-  Definition exec_triple_addr {Σ : World}
-    (req : Assertion (Σ ▻ ("a"::ty_xlenbits))) (b : list AnnotInstr)
-    (ens : Assertion (Σ ▻ ("a"::ty_xlenbits) ▻ ("an"::ty_xlenbits))) : M Unit Σ :=
-    ω1 ∣ a <- @demonic _ _ ;;
-    ω2 ∣ _ <- produce req (sub_snoc (sub_acc ω1) _ a) ;;
-    ω3 ∣ na <- @exec_block_addr b _ (persist__term a ω2) (persist__term a ω2) ;;
-    consume ens
-      (sub_snoc (sub_snoc (sub_acc (ω1 ∘ ω2 ∘ ω3)) _ (persist__term a (ω2 ∘ ω3))) ("an"::ty_xlenbits) na).
+    Definition exec_instruction_epilogue (i : AST) :
+      Assertion ([ctx] ▻ ("a":: ty_xlenbits) ▻ ("an":: ty_xlenbits)) :=
+      pc     ↦ term_var "an" ∗
+      asn.chunk (chunk_user ptstoinstr [term_var "a"; term_val ty_ast i]) ∗
+      nextpc ↦ term_var "an".
 
-  (* This is a VC for triples, for doubles we probably need to talk *)
-  (*    about the continuation of a block. *)
-  Definition VC__addr {Σ : LCtx} (req : Assertion {| wctx := Σ ▻ ("a":: ty_xlenbits); wco := []%ctx |}) (b : list AnnotInstr)
-    (ens : Assertion {| wctx := Σ ▻ ("a"::ty_xlenbits) ▻ ("an"::ty_xlenbits); wco := []%ctx |}) : 𝕊 ε :=
-    SymProp.demonic_close
-      (@exec_triple_addr
-         {| wctx := Σ; wco := []%ctx |}
-         req b ens
-         (* Could include leakcheck here *)
-         (fun _ _ _ _ h => SymProp.block)
-         []%env []%list).
-End BlockVerification3.
+    Definition sexec_instruction (i : AST) :
+      ⊢ STerm ty_xlenbits -> SHeapSpec (STerm ty_xlenbits) :=
+      let inline_fuel := 10%nat in
+      fun _ a =>
+        ⟨ θ1 ⟩ _  <- produce
+                       (exec_instruction_prologue i)
+                       [env].["a"∷_ ↦ a] ;;
+        ⟨ θ2 ⟩ _  <- evalStoreSpec (exec default_config inline_fuel (FunDef step)) [env] ;;
+        ⟨ θ3 ⟩ na <- angelic None _ ;;
+        let a3 := persist__term a (θ1 ∘ θ2 ∘ θ3) in
+        ⟨ θ4 ⟩ _  <- consume
+                       (exec_instruction_epilogue i)
+                       [env].["a"∷_ ↦ a3].["an"∷_ ↦ na] ;;
+        pure (persist__term na θ4).
 
-Module BlockVerificationDerived2Sound.
-  Import RiscvPmpBlockVerifSpec.
-  Import RiscvPmpBlockVerifShalExecutor.
-  Import RiscvPmpIrisInstanceWithContracts.
+    Fixpoint sexec_block_addr (b : list AST) :
+      ⊢ STerm ty_xlenbits -> STerm ty_xlenbits -> SHeapSpec (STerm ty_xlenbits) :=
+      fun _ ainstr apc =>
+        match b with
+        | nil       => pure apc
+        | cons i b' =>
+            ⟨ θ1 ⟩ _    <- assert_formula (fun _ => amsg.empty)
+                             (formula_relop bop.eq ainstr apc) ;;
+            ⟨ θ2 ⟩ apc' <- sexec_instruction i (persist__term apc θ1) ;;
+            sexec_block_addr b'
+              (term_binop bop.bvadd
+                 (persist__term ainstr (θ1 ∘ θ2))
+                 (term_val ty_word bv_instrsize))
+              apc'
+        end.
 
-  Definition M : Type -> Type := CStoreSpec [] [].
+    Definition sexec_double_addr {Σ : LCtx}
+      (req : Assertion (Σ ▻ ("a":: ty_xlenbits))) (b : list AST) :
+      ⊢ SHeapSpec (STerm ty_xlenbits) :=
+      fun _ =>
+        ⟨ θ1 ⟩ lenv1 <- demonic_ctx id Σ ;;
+        ⟨ θ2 ⟩ a2    <- demonic (Some "a") _ ;;
+        let lenv2 := env.snoc (persist (A := Sub Σ) lenv1 θ2) _ a2 in
+        ⟨ θ3 ⟩ _     <- produce req lenv2 ;;
+        let a3 := persist__term a2 θ3 in
+        sexec_block_addr b a3 a3.
 
-  Definition pure {A} : A -> M A := CStoreSpec.pure.
-  Definition bind {A B} : M A -> (A -> M B) -> M B := CStoreSpec.bind.
-  Definition angelic {σ} : M (Val σ) := @CStoreSpec.angelic [] σ.
-  Definition demonic {σ} : M (Val σ) := @CStoreSpec.demonic [] σ.
-  Definition assert : Prop -> M unit := CStoreSpec.assert_formula.
-  Definition assume : Prop -> M unit := CStoreSpec.assume_formula.
+    Definition sexec_triple_addr {Σ : LCtx}
+      (req : Assertion (Σ ▻ ("a"::ty_xlenbits))) (b : list AST)
+      (ens : Assertion (Σ ▻ ("a"::ty_xlenbits) ▻ ("an"::ty_xlenbits))) :
+      ⊢ SHeapSpec Unit :=
+      fun w =>
+        ⟨ θ0 ⟩ δ <- demonic_ctx id Σ ;;
+        ⟨ θ1 ⟩ a <- demonic (Some "a") _ ;;
+        let δ1 := env.snoc (persist ( A:= Sub Σ) δ θ1) _ a in
+        ⟨ θ2 ⟩ _ <- produce req δ1 ;;
+        let a2 := persist__term a θ2 in
+        ⟨ θ3 ⟩ na <- sexec_block_addr b a2 a2 ;;
+        let δ3 := persist δ1 (θ2 ∘ θ3) in
+        consume ens δ3.["an"∷ty_xlenbits ↦ na].
 
-  Definition produce_chunk : SCChunk -> M unit := CStoreSpec.produce_chunk.
-  Definition consume_chunk : SCChunk -> M unit := CStoreSpec.consume_chunk.
+    (* This is a VC for triples, for doubles we probably need to talk
+       about the continuation of a block. *)
+    Definition sblock_verification_condition {Σ : LCtx}
+      (req : Assertion (Σ ▻ "a"∷ty_xlenbits)) (b : list AST)
+      (ens : Assertion (Σ ▻ "a"∷ty_xlenbits ▻ "an"∷ty_xlenbits)) : ⊢ 𝕊 :=
+      fun w =>
+        (* SHeapSpec does not perform a leakcheck. We could include one here. *)
+        SHeapSpec.run (sexec_triple_addr req b ens (w := w)).
 
-  Definition produce {Σ} : Assertion Σ -> Valuation Σ -> M unit := CStoreSpec.produce.
-  Definition consume {Σ} : Assertion Σ -> Valuation Σ -> M unit := CStoreSpec.consume.
+  End Symbolic.
 
-  Notation "x <- ma ;; mb" :=
-    (bind ma (fun x => mb))
-      (at level 80, ma at level 90, mb at level 200, right associativity).
+  Section Shallow.
 
-  Definition exec_instruction_any__c (i : AST) : Val ty_xlenbits -> M (Val ty_xlenbits) :=
-    let inline_fuel := 10%nat in
-    fun a =>
-      _ <- produce_chunk (scchunk_ptsreg pc a) ;;
-      _ <- produce_chunk (scchunk_user ptstoinstr [a; i]) ;;
-      an <- @demonic _ ;;
-      _ <- produce_chunk (scchunk_ptsreg nextpc an) ;;
-      _ <- CStoreSpec.exec inline_fuel (FunDef step) ;;
-      _ <- consume_chunk (scchunk_user ptstoinstr [a ; i]) ;;
-      na <- @angelic _ ;;
-      _ <- consume_chunk (scchunk_ptsreg nextpc na) ;;
-      _ <- consume_chunk (scchunk_ptsreg pc na) ;; (* TODO: a + 4! *)
-      pure na.
+    Import CStoreSpec (evalStoreSpec, exec).
+    Import CHeapSpec CHeapSpec.notations.
 
-  Import logicalrelation logicalrelation.notations.
-  Import StoreSpec.
-  Import proofmode.
-  Import iris.proofmode.tactics.
+    Definition cexec_instruction (i : AST) :
+      Val ty_xlenbits -> CHeapSpec (Val ty_xlenbits) :=
+      let inline_fuel := 10%nat in
+      fun a =>
+        _ <- produce
+               (exec_instruction_prologue i)
+               [env].["a"∷_ ↦ a] ;;
+        _ <- evalStoreSpec (exec inline_fuel (FunDef step)) [env] ;;
+        na <- angelic _ ;;
+        _ <- consume
+               (exec_instruction_epilogue i)
+               [env].["a"∷ty_xlenbits ↦ a].["an"∷_ ↦ na] ;;
+        pure na.
 
-  Lemma refine_exec_instruction_any (i : AST) {w} :
-    ⊢ ℛ⟦RVal ty_xlenbits -> RStoreSpec [ctx] [ctx] (RVal ty_xlenbits)⟧
-      (exec_instruction_any__c i)
-      (BlockVerificationDerived2.exec_instruction_any (w := w) i).
-  Proof.
-    unfold BlockVerificationDerived2.exec_instruction_any, exec_instruction_any__c.
-    now rsolve.
-  Qed.
+    Fixpoint cexec_block_addr (b : list AST) :
+      Val ty_xlenbits -> Val ty_xlenbits -> CHeapSpec (Val ty_xlenbits) :=
+      fun ainstr apc =>
+        match b with
+        | nil       => pure apc
+        | cons i b' =>
+            _ <- assert_formula (ainstr = apc) ;;
+            apc' <- cexec_instruction i apc ;;
+            cexec_block_addr b' (bv.add ainstr bv_instrsize) apc'
+        end.
 
-  #[export] Instance refine_compat_exec_instruction_any {i : AST} {w} :
-    RefineCompat (RVal ty_xlenbits -> RStoreSpec [ctx] [ctx] (RVal ty_xlenbits))
-      (exec_instruction_any__c i) w (BlockVerificationDerived2.exec_instruction_any (w := w) i) _ :=
-    MkRefineCompat (refine_exec_instruction_any i).
+    Definition cexec_double_addr {Σ : LCtx}
+      (req : Assertion (Σ ▻ "a"∷ty_xlenbits)) (b : list AST) :
+      CHeapSpec (Val ty_xlenbits) :=
+      δ <- demonic_ctx Σ ;;
+      an <- demonic _ ;;
+      _ <- produce req δ.["a"∷ty_xlenbits ↦ an] ;;
+      cexec_block_addr b an an.
 
-  Fixpoint exec_block_addr__c (b : list AST) : Val ty_xlenbits -> Val ty_xlenbits -> M (Val ty_xlenbits) :=
-    fun ainstr apc =>
-      match b with
-      | nil       => pure apc
-      | cons i b' =>
-          _ <- assert (ainstr = apc) ;;
-          apc' <- exec_instruction_any__c i apc ;;
-          @exec_block_addr__c b' (bv.add ainstr bv_instrsize) apc'
-      end.
+    Definition cexec_triple_addr {Σ : LCtx}
+      (req : Assertion (Σ ▻ "a"∷ty_xlenbits)) (b : list AST)
+      (ens : Assertion (Σ ▻ "a"∷ty_xlenbits ▻ "an"∷ty_xlenbits)) :
+      CHeapSpec unit :=
+      lenv <- demonic_ctx Σ ;;
+      a    <- demonic _ ;;
+      _    <- produce req lenv.["a"∷ty_xlenbits ↦ a]  ;;
+      na   <- cexec_block_addr b a a ;;
+      consume ens lenv.["a"∷ty_xlenbits ↦ a].["an"∷ty_xlenbits ↦ na].
 
-  Lemma refine_exec_block_addr (b : list AST) {w} :
-    ⊢ ℛ⟦RVal ty_xlenbits -> RVal ty_xlenbits -> RStoreSpec [ctx] [ctx] (RVal ty_xlenbits)⟧
-      (exec_block_addr__c b)
-      (@BlockVerificationDerived2.exec_block_addr b w).
-  Proof.
-    iAssert (ℛ⟦□ᵣ (RVal ty_xlenbits -> RVal ty_xlenbits -> RStoreSpec [ctx] [ctx] (RVal ty_xlenbits))⟧
-               (exec_block_addr__c b)
-               (fun w' ω => @BlockVerificationDerived2.exec_block_addr b w')) as "H".
-    { 
-      unfold exec_block_addr__c, BlockVerificationDerived2.exec_block_addr.
-      iInduction b as [|*] "IHb"; rsolve.
-      iApply ("IHb" with "[] [$]").
-      now rsolve.
-    } 
-    iApply (unconditionally_T with "H").
-  Qed.
+    Definition cblock_verification_condition {Σ : LCtx}
+      (req : Assertion (Σ ▻ "a"∷ty_xlenbits)) (b : list AST)
+      (ens : Assertion (Σ ▻ "a"∷ty_xlenbits ▻ "an"∷ty_xlenbits)) : Prop :=
+      (* CHeapSpec.run does not perform a leakcheck. We could include one here. *)
+      CHeapSpec.run (cexec_triple_addr req b ens).
 
-  Definition exec_double_addr__c {Σ : World} (ι : Valuation Σ)
-    (req : Assertion (wsnoc Σ ("a"∷ty_xlenbits))) (b : list AST) : M (Val ty_xlenbits) :=
-    an <- @demonic _ ;;
-    _ <- produce req (env.snoc ι ("a"::ty_xlenbits) an)  ;;
-    @exec_block_addr__c b an an.
+    #[export] Instance mon_eval_exec {Γ τ} n (s : Stm Γ τ) δ :
+      Monotonic (MHeapSpec eq) (CStoreSpec.evalStoreSpec (CStoreSpec.exec n s) δ).
+    Proof.
+      intros P Q PQ h. unfold Basics.impl, CStoreSpec.evalStoreSpec.
+      apply RiscvPmpIrisInstanceWithContracts.exec_monotonic.
+      intros ? ? ?. now apply PQ.
+    Qed.
 
-  Definition exec_triple_addr__c {Σ : LCtx} (ι : Valuation Σ)
-    (req : Assertion (Σ ▻ ("a"::ty_xlenbits))) (b : list AST)
-    (ens : Assertion (Σ ▻ ("a"::ty_xlenbits) ▻ ("an"::ty_xlenbits))) : M unit :=
-    a <- @demonic _ ;;
-    _ <- produce req (ι ► ( _ ↦ a ))  ;;
-    na <- @exec_block_addr__c b a a ;;
-    consume ens (ι ► ( ("a"::ty_xlenbits) ↦ a ) ► ( ("an"::ty_xlenbits) ↦ na )).
+    #[export] Instance mono_cexec_instruction {i a} :
+      Monotonic (MHeapSpec eq) (cexec_instruction i a).
+    Proof. typeclasses eauto. Qed.
 
-  Import ModalNotations.
+    #[export] Instance mono_cexec_block_addr {instrs ainstr apc} :
+      Monotonic (MHeapSpec eq) (cexec_block_addr instrs ainstr apc).
+    Proof. revert ainstr apc. induction instrs; cbn; typeclasses eauto. Qed.
 
-  Lemma refine_exec_triple_addr {Σ : LCtx}
-    (req : Assertion (Σ ▻ ("a"::ty_xlenbits))) (b : list AST)
-    (ens : Assertion (Σ ▻ ("a"::ty_xlenbits) ▻ ("an"::ty_xlenbits)))
-    (ι : Valuation Σ) :
-    ⊢ forgetting (acc_wlctx_valuation ι)
-      (ℛ⟦RStoreSpec [ctx] [ctx] RUnit⟧
-         (exec_triple_addr__c ι req b ens)
-         (@BlockVerificationDerived2.exec_triple_addr (wlctx Σ) req b ens)).
-  Proof.
-    unfold BlockVerificationDerived2.exec_triple_addr, exec_triple_addr__c.
-    iPoseProof (forgetting_valuation_repₚ (w := wlctx Σ) ι (sub_id Σ)) as "#Hιs".
-    rewrite inst_sub_id.
-    iModIntro.
-    rsolve.
-    - rewrite <-forgetting_repₚ.
-      now rewrite persist_subst sub_comp_id_left.
-    - iApply refine_exec_block_addr;
+  End Shallow.
+
+  Section Relational.
+
+    Import iris.proofmode.tactics logicalrelation logicalrelation.notations.
+    Import RiscvPmpIrisInstanceWithContracts.StoreSpec.
+    Import RiscvPmpSignature.HeapSpec.
+
+    Lemma rexec_instruction (i : AST) {w} :
+      ⊢ ℛ⟦RVal ty_xlenbits -> RHeapSpec (RVal ty_xlenbits)⟧
+          (cexec_instruction i)
+          (sexec_instruction (w := w) i).
+    Proof.
+      unfold cexec_instruction, sexec_instruction. rsolve.
+      all: iApply refine_namedenv_nil.
+    Qed.
+
+    #[export] Instance refine_compat_exec_instruction {i : AST} {w} :
+      RefineCompat (RVal ty_xlenbits -> RHeapSpec (RVal ty_xlenbits))
+        (cexec_instruction i) w (sexec_instruction (w := w) i) _ :=
+      MkRefineCompat (rexec_instruction i).
+
+    Lemma rexec_block_addr (b : list AST) {w} :
+      ⊢ ℛ⟦RVal ty_xlenbits -> RVal ty_xlenbits -> RHeapSpec (RVal ty_xlenbits)⟧
+          (cexec_block_addr b)
+          (sexec_block_addr b (w := w)).
+    Proof.
+      iAssert (ℛ⟦□ᵣ (RVal ty_xlenbits -> RVal ty_xlenbits -> RHeapSpec (RVal ty_xlenbits))⟧
+                 (cexec_block_addr b)
+                 (fun w' θ => sexec_block_addr b (w := w'))) as "H".
+      {
+        iInduction b as [|*] "IHb"; cbn; rsolve.
+        iApply HeapSpec.refine_assert_formula.
         rsolve.
-    - rewrite forgetting_trans.
-      iModIntro.
-      rewrite <-forgetting_repₚ.
-      now rewrite persist_subst sub_comp_id_left.
-  Qed.
-
-End BlockVerificationDerived2Sound.
-
-Module BlockVerification3Sound.
-  Import RiscvPmpBlockVerifSpec.
-  Import RiscvPmpBlockVerifShalExecutor.
-  Import RiscvPmpIrisInstanceWithContracts.
-  Import BlockVerificationDerived2.
-  Import BlockVerification3.
-  Import BlockVerificationDerived2Sound.
-
-  Fixpoint exec_block_addr__c (b : list AnnotInstr) : Val ty_xlenbits -> Val ty_xlenbits -> M (Val ty_xlenbits) :=
-    fun ainstr apc =>
-      match b with
-      | nil       => pure apc
-      | cons instr b' =>
-          match instr with
-          | AnnotAST i => _ <- assert (ainstr = apc) ;;
-                         apc' <- exec_instruction_any__c i apc ;;
-                         @exec_block_addr__c b' (bv.add ainstr bv_instrsize) apc'
-          | AnnotDebugBreak => pure apc
-          | AnnotLemmaInvocation l es =>
-              args <- CStoreSpec.eval_exps es ;;
-              _ <- CStoreSpec.call_lemma (LEnv l) args ;;
-              exec_block_addr__c b' ainstr apc
-          end
-      end.
-
-  Import logicalrelation logicalrelation.notations.
-  Import iris.bi.interface iris.proofmode.tactics.
-  Import StoreSpec.
-  Import proofmode.
-
-  Lemma refine_exec_block_addr (b : list AnnotInstr) {w} :
-    ⊢ ℛ⟦RVal ty_xlenbits -> RVal ty_xlenbits -> RStoreSpec [ctx] [ctx] (RVal ty_xlenbits)⟧
-      (exec_block_addr__c b)
-      (@BlockVerification3.exec_block_addr b w).
-  Proof.
-    iAssert (ℛ⟦□ᵣ (RVal ty_xlenbits -> RVal ty_xlenbits -> RStoreSpec [ctx] [ctx] (RVal ty_xlenbits))⟧
-               (exec_block_addr__c b)
-               (fun w ω => @BlockVerification3.exec_block_addr b w)) as "H".
-    { iInduction b as [|instr b] "IHb"; rsolve.
-      destruct instr; cbn; rsolve.
-      - iApply "IHb"; rsolve; now rewrite ?sub_acc_trans.
-      - iApply "IHb"; rsolve; now rewrite ?sub_acc_trans. }
-    now iApply (unconditionally_T with "H").
-  Qed.
-
-  Definition exec_triple_addr__c {Σ : World} (ι : Valuation Σ)
-    (req : Assertion (Σ ▻ ("a"::ty_xlenbits))) (b : list AnnotInstr)
-    (ens : Assertion (Σ ▻ ("a"::ty_xlenbits) ▻ ("an"::ty_xlenbits))) : M unit :=
-    a <- @demonic _ ;;
-    _ <- produce req (ι ► ( _ ↦ a )) ;;
-    na <- @exec_block_addr__c b a a ;;
-    consume ens (ι ► ( ("a"::ty_xlenbits) ↦ a ) ► ( ("an"::ty_xlenbits) ↦ na )).
-
-  Import ModalNotations.
-
-  Lemma refine_exec_triple_addr {Σ : LCtx}
-    (req : Assertion (Σ ▻ ("a"::ty_xlenbits))) (b : list AnnotInstr)
-    (ens : Assertion (Σ ▻ ("a"::ty_xlenbits) ▻ ("an"::ty_xlenbits))) (ι : Valuation Σ) :
-    ⊢ forgetting (acc_wlctx_valuation ι)
-      (ℛ⟦RStoreSpec [ctx] [ctx] RUnit⟧
-         (exec_triple_addr__c (Σ := wlctx Σ) ι req b ens)
-         (@BlockVerification3.exec_triple_addr (wlctx Σ) req b ens)).
-  Proof.
-    iPoseProof (forgetting_valuation_repₚ (w := wlctx Σ) ι (sub_id Σ)) as "#Hιs".
-    unfold BlockVerification3.exec_triple_addr, exec_triple_addr__c.
-    iModIntro.
-    rsolve.
-    - rewrite inst_sub_id.
-      now iApply refine_namedenv_sub_acc.
-    - iApply refine_exec_block_addr; now rsolve.
-    - rewrite forgetting_trans.
-      iModIntro.
-      rewrite inst_sub_id.
-      now iApply refine_namedenv_sub_acc.
-  Qed.
-
-End BlockVerification3Sound.
-
-Module BlockVerificationDerived2Sem.
-  Import iris.program_logic.weakestpre.
-  Import iris.proofmode.tactics.
-  Import RiscvPmpBlockVerifSpec.
-  Import BlockVerificationDerived2.
-  Import Shallow.Executor.
-  Import ctx.resolution.
-  Import ctx.notations.
-  Import env.notations.
-  Import RiscvPmpIrisBase.
-  Import RiscvPmpIrisInstance.
-  Import RiscvPmpIrisInstanceWithContracts.
-  Import RiscvPmpBlockVerifShalExecutor.
-  Import BlockVerificationDerived2Sound.
-
-  Definition semTripleOneInstrStep `{sailGS Σ} (PRE : iProp Σ) (instr : AST) (POST : Val ty_word -> iProp Σ) (a : Val ty_word) : iProp Σ :=
-    semTriple [] (PRE ∗ (∃ v, lptsreg nextpc v) ∗ lptsreg pc a ∗ interp_ptsto_instr a instr)
-      (FunDef RiscvPmpProgram.step)
-      (fun ret _ => (∃ an, lptsreg nextpc an ∗ lptsreg pc an ∗ POST an) ∗ interp_ptsto_instr a instr)%I.
-
-  Lemma mono_exec_instruction_any__c {i a} : Monotonic' (exec_instruction_any__c i a).
-  Proof.
-    cbv [Monotonic' exec_instruction_any__c bind CStoreSpec.bind produce_chunk CStoreSpec.produce_chunk demonic CStoreSpec.demonic angelic CStoreSpec.angelic pure CStoreSpec.pure].
-    intros δ P Q PQ h eP v.
-    destruct (env.view δ).
-    specialize (eP v); revert eP.
-    apply exec_monotonic.
-    clear -PQ. intros _ δ h.
-    destruct (env.view δ).
-    apply consume_chunk_monotonic.
-    clear -PQ. intros _ h.
-    intros [v H]; exists v; revert H.
-    apply consume_chunk_monotonic.
-    clear -PQ; intros _ h.
-    apply consume_chunk_monotonic.
-    clear -PQ; intros _ h.
-    now apply PQ.
-  Qed.
-
-  Lemma sound_stm_aux `{sailGS Σ} {τ} {PRE} {s : Stm [ctx] τ} {POST} :
-    ProgramLogic.Triple [env] PRE s POST ->
-    ⊢ semTriple [env] PRE s POST.
-  Proof.
-    iIntros (Htrip) "PRE".
-    iApply wp_mono.
-    2: {
-      iApply sound_stm.
-      - apply foreignSemBlockVerif.
-      - apply lemSemBlockVerif.
-      - apply Htrip.
-      - iApply contractsSound.
-      - iFrame.
-    }
-    now iIntros.
-  Qed.
-
-  Lemma sound_exec_instruction_any_aux `{sailGS Σ} {instr} (h : SCHeap) (POST : Val ty_xlenbits -> CStore [ctx] -> iProp Σ) :
-    forall a npc,
-    exec_instruction_any__c instr a (fun res => liftP (POST res)) [] h ->
-    ProgramLogic.Triple []
-      (interpret_scheap (scchunk_ptsreg nextpc npc :: scchunk_user ptstoinstr [a; instr] :: scchunk_ptsreg pc a :: h)%list)
-      (FunDef RiscvPmpProgram.step)
-      (fun res => (fun δ' => interp_ptsto_instr a instr ∗ (∃ v, lptsreg nextpc v ∗ lptsreg pc v ∗ POST v δ'))%I).
-  Proof.
-    cbv [exec_instruction_any__c bind CStoreSpec.bind produce_chunk consume_chunk
-      CStoreSpec.produce_chunk CHeapSpec.produce_chunk CPureSpec.produce_chunk
-      CPureSpec.pure demonic CStoreSpec.demonic CStoreSpec.lift_purem
-      CPureSpec.demonic].
-    intros a npc Htrip. specialize (Htrip npc).
-    apply (exec_sound 10). revert Htrip.
-    apply exec_monotonic.
-    intros _ δ0 h0 HYP.
-    refine (consume_chunk_sound (scchunk_user ptstoinstr [a; instr]) (fun δ' => (∃ v, lptsreg nextpc v ∗ lptsreg pc v ∗ POST v δ'))%I δ0 h0 _).
-    revert HYP. apply consume_chunk_monotonic.
-    intros _ h1 [an Hrest]; revert Hrest.
-    cbn.
-    iIntros (HYP') "Hh1".
-    iExists an.
-    iStopProof.
-    refine (consume_chunk_sound (scchunk_ptsreg nextpc an) (fun δ' => lptsreg pc an ∗ POST an δ')%I δ0 h1 _).
-    revert HYP'.
-    apply consume_chunk_monotonic.
-    intros _ h2 HYP2.
-    refine (consume_chunk_sound (scchunk_ptsreg pc an) (fun δ' => POST an δ')%I δ0 h2 _).
-    revert HYP2.
-    apply consume_chunk_monotonic.
-    now intros _ h3 HYP3.
-  Qed.
-
-
-  Lemma sound_exec_instruction_any `{sailGS Σ} {instr} (h : SCHeap) (POST : Val ty_xlenbits -> CStore [ctx] -> iProp Σ) :
-    forall a,
-    exec_instruction_any__c instr a (fun res => liftP (POST res)) [] h ->
-    ⊢ semTripleOneInstrStep (interpret_scheap h) instr (fun an => POST an []) a.
-  Proof.
-    intros a.
-    intros Hverif.
-    iIntros "(Hheap & [%npc Hnpc] & Hpc & Hinstrs)".
-    apply (sound_exec_instruction_any_aux _ npc) in Hverif.
-    iApply (semWP_mono with "[-]").
-    iApply (sound_stm_aux Hverif with "[$Hnpc $Hinstrs $Hpc $Hheap]").
-    iIntros ([] store) "[Hinstr [%an (Hnextpc & Hpc & HPOST)]]".
-    destruct (env.view store).
-    iFrame.
-    iExists an.
-    iFrame.
-  Qed.
-
-  Notation "a '↦' t" := (reg_pointsTo a t) (at level 70).
-  Notation "a '↦ₘ' t" := (interp_ptsto a t) (at level 70).
-
-  Fixpoint ptsto_instrs `{sailGS Σ} (a : Val ty_word) (instrs : list AST) : iProp Σ :=
-    match instrs with
-    | cons inst insts => (interp_ptsto_instr a inst ∗ ptsto_instrs (bv.add a bv_instrsize) insts)%I
-    | nil => True%I
-    end.
-  (* Arguments ptsto_instrs {Σ H} a%Z_scope instrs%list_scope : simpl never. *)
-
-  Lemma mono_exec_block_addr {instrs ainstr apc} : Monotonic' (exec_block_addr__c instrs ainstr apc).
-  Proof.
-    revert ainstr apc.
-    induction instrs; cbn.
-    - intros ainstr apc δ P Q PQ h.
-      cbv [pure CStoreSpec.pure].
-      apply PQ.
-    - intros ainstr apc.
-      cbv [Monotonic' bind CStoreSpec.bind assert CStoreSpec.assert_formula CStoreSpec.lift_purem CPureSpec.assert_formula].
-      intros δ P Q PQ h [<- Hverif].
-      split; [reflexivity|].
-      revert Hverif.
-      apply mono_exec_instruction_any__c.
-      intros res h2.
-      apply IHinstrs.
-      intros res2 h3.
-      now apply PQ.
-  Qed.
-
-  Lemma sound_exec_block_addr `{sailGS Σ} {instrs ainstr apc} (h : SCHeap) (POST : Val ty_xlenbits -> CStore [ctx] -> iProp Σ) :
-    exec_block_addr__c instrs ainstr apc (fun res => liftP (POST res)) [] h ->
-    ⊢ ((interpret_scheap h ∗ lptsreg pc apc ∗ (∃ v, lptsreg nextpc v) ∗ ptsto_instrs ainstr instrs) -∗
-            (∀ an, lptsreg pc an ∗ (∃ v, lptsreg nextpc v) ∗ ptsto_instrs ainstr instrs ∗ POST an [] -∗ WP_loop) -∗
-            WP_loop)%I.
-  Proof.
-    revert ainstr apc h POST.
-    induction instrs as [|instr instrs]; cbn; intros ainstr apc h POST.
-    - iIntros (Hverif) "(Hpre & Hpc & Hnpc & _) Hk".
-      iApply "Hk"; iFrame.
-      iSplitR; auto.
-      now iApply Hverif.
-    - intros [-> Hverif].
-      iIntros "(Hh & Hpc & Hnpc & Hinstr & Hinstrs) Hk".
-      iApply semWP_seq.
-      iApply semWP_call_inline.
-      cbn.
-      iApply (semWP_mono with "[-Hinstrs Hk] [Hinstrs Hk]").
-      { iApply (sound_exec_instruction_any (fun an δ => (lptsreg pc an) ∗ (∃ v, lptsreg nextpc v) ∗ ptsto_instrs (bv.add apc bv_instrsize) instrs -∗ (∀ an2 : Val ty_word, pc ↦ an2 ∗ (∃ v, nextpc ↦ v) ∗ ptsto_instrs (bv.add apc bv_instrsize) instrs ∗ POST an2 [env] -∗ WP_loop) -∗ WP_loop)%I with "[$]").
-        revert Hverif.
-        apply mono_exec_instruction_any__c.
-        intros an h2.
-        unfold liftP; cbn.
-        iIntros (Hverif) "Hh2 (Hpc & Hnpc & Hinstrs) Hk".
-        iApply (IHinstrs (bv.add apc bv_instrsize)%Z an _ _ Hverif with "[$]").
-        iIntros (an2) "(Hpc & Hinstrs & HPOST)".
-        iApply ("Hk" with "[$]").
+        iApply ("IHb" with "[] [$]").
+        now rsolve.
       }
-      iIntros (_ _) "([%an (Hnpc & Hpc & Hk2)] & Hinstr)".
-      iSpecialize ("Hk2" with "[$Hpc Hnpc $Hinstrs]").
-      { now iExists an. }
-      iApply (semWP_call_inline loop).
-      iApply "Hk2".
-      iIntros (an2) "(Hpc & Hnpc & Hinstrs & HPOST)".
-      iApply ("Hk" with "[$]").
-  Qed.
+      iApply (unconditionally_T with "H").
+    Qed.
 
-  Definition semTripleBlock `{sailGS Σ} (PRE : Val ty_word -> iProp Σ) (instrs : list AST) (POST : Val ty_word -> Val ty_word -> iProp Σ) : iProp Σ :=
-    (∀ a,
-    (PRE a ∗ pc ↦ a ∗ (∃ v, nextpc ↦ v) ∗ ptsto_instrs a instrs) -∗
-      (∀ an, pc ↦ an ∗ (∃ v, nextpc ↦ v) ∗ ptsto_instrs a instrs ∗ POST a an -∗ WP_loop) -∗
-      WP_loop)%I.
-  Global Arguments semTripleBlock {Σ} {_} PRE%I instrs POST%I.
+    Lemma rexec_triple_addr {Σ : LCtx}
+      (req : Assertion (Σ ▻ "a"∷ty_xlenbits)) (b : list AST)
+      (ens : Assertion (Σ ▻ "a"∷ty_xlenbits ▻ "an"∷ty_xlenbits)) {w} :
+      ⊢ ℛ⟦RHeapSpec RUnit⟧
+          (cexec_triple_addr req b ens)
+          (sexec_triple_addr req b ens (w := w)).
+    Proof.
+      unfold cexec_triple_addr, sexec_triple_addr.
+      rsolve.
+      iApply rexec_block_addr; rsolve.
+      rewrite !forgetting_trans.
+      iModIntro.
+      iModIntro.
+      rsolve.
+    Qed.
 
-  Lemma sound_exec_triple_addr__c `{sailGS Σ} {W : World} {pre post instrs} {ι : Valuation W} :
-      (exec_triple_addr__c ι pre instrs post (λ _ _ _ , True) [env] []%list) ->
-    ⊢ semTripleBlock (λ a : Val ty_word, asn.interpret pre (ι.[("a"::ty_xlenbits) ↦ a])) instrs
-      (λ a na : Val ty_word, asn.interpret post (ι.[("a"::ty_xlenbits) ↦ a].[("an"::ty_xlenbits) ↦ na])).
-  Proof.
-    intros Hexec.
-    iIntros (a) "(Hpre & Hpc & Hnpc & Hinstrs) Hk".
-    specialize (Hexec a).
-    unfold bind, CStoreSpec.bind, produce, CStoreSpec.produce, CStoreSpec.lift_heapspec in Hexec.
-    apply CHeapSpec.produce_sound in Hexec.
-    iPoseProof (Hexec with "[//] Hpre") as "(%h & Hh & %Hexec')". clear Hexec.
-    iApply (sound_exec_block_addr h
-                  (fun an δ => asn.interpret post ι.["a"∷ty_word ↦ a].["an"∷ty_word ↦ an])%I
-             with "[$Hh $Hpc $Hnpc $Hinstrs] Hk").
-    revert Hexec'.
-    apply mono_exec_block_addr.
-    intros res h2 Hcons. cbn.
-    unfold liftP.
-    rewrite <- (bi.sep_True (asn.interpret _ _)).
-    iApply consume_sound.
-    revert Hcons.
-    apply CHeapSpec.mon_consume.
-    intros _ _ _ h3 _. auto.
-  Qed.
+    Lemma rblock_verification_condition {Σ : LCtx}
+      (req : Assertion (Σ ▻ "a"∷ty_xlenbits)) (b : list AST)
+      (ens : Assertion (Σ ▻ "a"∷ty_xlenbits ▻ "an"∷ty_xlenbits)) {w} :
+      ⊢ RSat LogicalSoundness.RProp (w := w)
+          (cblock_verification_condition req b ens)
+          (sblock_verification_condition req b ens w).
+    Proof.
+      unfold cblock_verification_condition, sblock_verification_condition.
+      rsolve.
+      iApply refine_run.
+      iApply rexec_triple_addr.
+    Qed.
 
-  Lemma sound_VC__addr `{sailGS Σ} {Γ} {pre post instrs} :
-    safeE (postprocess (BlockVerificationDerived2.VC__addr (Σ := Γ) pre instrs post)) ->
-    forall ι,
-    ⊢ semTripleBlock (fun a => asn.interpret pre (ι.[("a"::ty_xlenbits) ↦ a]))
-      instrs
-      (fun a na => asn.interpret post (ι.[("a"::ty_xlenbits) ↦ a].[("an"::ty_xlenbits) ↦ na])).
-  Proof.
-    intros Hverif ι.
-    apply (sound_exec_triple_addr__c (W := {| wctx := Γ ; wco := []%ctx |}) (pre := pre) (post := post) (instrs := instrs)).
-    eapply (fromEntails (w := wnil) (refine_exec_triple_addr (Σ := wlctx Γ) _ _ _ ι) [env] I I).
-    - done.
-    - eapply refine_lift; now cbn.
-    - now eapply logicalrelation.rlist_nil.
-    - rewrite inst_lift.
-      apply (fromBientails (w := wlctx Γ) LogicalSoundness.psafe_safe ι I).
-      apply (safeE_safe env.nil), postprocess_sound in Hverif.
-      rewrite SymProp.safe_demonic_close in Hverif.
-      now apply Hverif.
-  Qed.
+  End Relational.
 
-End BlockVerificationDerived2Sem.
+  Section Soundness.
 
-Module BlockVerification3Sem.
-  Import iris.program_logic.weakestpre.
-  Import iris.proofmode.tactics.
-  Import RiscvPmpBlockVerifSpec.
-  Import BlockVerificationDerived2.
-  Import Shallow.Executor.
-  Import ctx.resolution.
-  Import ctx.notations.
-  Import env.notations.
-  Import RiscvPmpIrisBase.
-  Import RiscvPmpIrisInstance.
-  Import RiscvPmpIrisInstanceWithContracts.
-  Import RiscvPmpBlockVerifShalExecutor.
-  Import BlockVerificationDerived2Sound.
-  Import BlockVerificationDerived2Sem.
-  Import BlockVerification3.
-  Import BlockVerification3Sound.
+    Import iris.base_logic.lib.iprop iris.proofmode.tactics.
+    Import RiscvPmpIrisInstanceWithContracts.
+    Import ProgramLogic.
+    Import CHeapSpec.
 
-  Lemma mono_exec_block_addr {instrs ainstr apc} : Monotonic' (exec_block_addr__c instrs ainstr apc).
-  Proof.
-    revert ainstr apc.
-    induction instrs as [|instr instrs]; cbn.
-    - intros ainstr apc δ P Q PQ h.
-      cbv [pure CStoreSpec.pure].
-      apply PQ.
-    - destruct instr.
-      + intros ainstr apc.
-        cbv [Monotonic' bind CStoreSpec.bind assert CStoreSpec.assert_formula CStoreSpec.lift_purem CPureSpec.assert_formula].
-        intros δ P Q PQ h [<- Hverif].
-        split; [reflexivity|].
-        revert Hverif.
-        apply mono_exec_instruction_any__c.
-        intros res h2.
-        apply IHinstrs.
-        intros res2 h3.
-        now apply PQ.
-      + intros ainstr apc.
-        cbv [Monotonic' pure CStoreSpec.pure].
-        intros. now apply PQ.
-      + intros ainstr apc.
-        cbv [Monotonic' bind CStoreSpec.bind assert CStoreSpec.assert_formula CStoreSpec.lift_purem CPureSpec.assert_formula].
-        intros δ P Q PQ h.
-        apply call_lemma_monotonic.
-        intros res δ1 h2.
-        apply IHinstrs.
-        intros res2 h3.
-        destruct (env.view δ), (env.view δ1).
-        now apply PQ.
-  Qed.
+    Context {Σ} {GS : sailGS Σ}.
 
-  Definition extract_AST (i : AnnotInstr) : option AST :=
-    match i with
-    | AnnotAST a => Some a
-    | _ => None
-    end.
+    Fixpoint ptsto_instrs (a : Val ty_word) (instrs : list AST) : iProp Σ :=
+      match instrs with
+      | cons inst insts => (interp_ptsto_instr a inst ∗ ptsto_instrs (bv.add a bv_instrsize) insts)%I
+      | nil => True%I
+      end.
+    (* Arguments ptsto_instrs {Σ H} a%Z_scope instrs%list_scope : simpl never. *)
 
-  Lemma sound_exec_block_addr `{sailGS Σ} {instrs ainstr apc} (h : SCHeap) (POST : Val ty_xlenbits -> CStore [ctx] -> iProp Σ) :
-    LemmaSem ->
-    exec_block_addr__c instrs ainstr apc (fun res => liftP (POST res)) [] h ->
-    ⊢ ((interpret_scheap h ∗ lptsreg pc apc ∗ (∃ v, lptsreg nextpc v) ∗ ptsto_instrs ainstr (omap extract_AST instrs)) -∗
-            (∀ an, lptsreg pc an ∗ (∃ v, lptsreg nextpc v) ∗ ptsto_instrs ainstr (omap extract_AST instrs) ∗ POST an [] -∗ WP_loop) -∗
-            WP_loop)%I.
-  Proof.
-    intros lemSem.
-    revert ainstr apc h POST.
-    induction instrs as [|instr instrs]; cbn; intros ainstr apc h POST.
-    - iIntros (Hverif) "(Hpre & Hpc & Hnpc & _) Hk".
-      iApply "Hk"; iFrame.
-      iSplitR; auto.
-      now iApply Hverif.
-    - destruct instr as [instr| |Δ lem es].
-      + intros [-> Hverif].
+    Definition semTripleOneInstrStep (PRE : iProp Σ) (instr : AST) (POST : Val ty_word -> iProp Σ) (a : Val ty_word) : iProp Σ :=
+      semTriple [env] (PRE ∗ (∃ v, lptsreg nextpc v) ∗ lptsreg pc a ∗ interp_ptsto_instr a instr)
+        (FunDef RiscvPmpProgram.step)
+        (fun ret _ => (∃ an, lptsreg nextpc an ∗ lptsreg pc an ∗ POST an) ∗ interp_ptsto_instr a instr)%I.
+
+    Definition semTripleBlock (PRE : Val ty_word -> iProp Σ) (instrs : list AST) (POST : Val ty_word -> Val ty_word -> iProp Σ) : iProp Σ :=
+      (∀ a,
+         (PRE a ∗ pc ↦ a ∗ (∃ v, nextpc ↦ v) ∗ ptsto_instrs a instrs) -∗
+         (∀ an, pc ↦ an ∗ (∃ v, nextpc ↦ v) ∗ ptsto_instrs a instrs ∗ POST a an -∗ WP_loop) -∗
+         WP_loop)%I.
+    #[global] Arguments semTripleBlock PRE%I instrs POST%I.
+
+    Lemma sound_stm_aux {τ} {PRE} {s : Stm [ctx] τ} {POST} :
+      ⦃ PRE ⦄ s; [env] ⦃ POST ⦄ → ⊢ semTriple [env] PRE s POST.
+    Proof.
+      iIntros (Htrip) "PRE".
+      iApply sound_stm; eauto using foreignSemBlockVerif, lemSemBlockVerif.
+      iApply contractsSound.
+    Qed.
+
+    Lemma sound_exec_instruction {instr} a Φ (h : SCHeap) :
+      cexec_instruction instr a Φ h ->
+      ⊢ semTripleOneInstrStep (interpret_scheap h) instr
+          (fun an => ∃ h' : SCHeap, interpret_scheap h' ∧ ⌜Φ an h'⌝) a.
+    Proof.
+      cbv [cexec_instruction exec_instruction_prologue bind produce demonic
+             produce_chunk lift_purespec CPureSpec.produce_chunk CPureSpec.pure
+             CPureSpec.demonic CStoreSpec.evalStoreSpec].
+      cbn - [consume].
+      iIntros (Hverif) "(Hheap & [%npc Hnpc] & Hpc & Hinstrs)".
+      specialize (Hverif npc). apply exec_sound_forwards in Hverif.
+      iApply (semWP_mono with "[-]").
+      iApply (sound_stm foreignSemBlockVerif lemSemBlockVerif Hverif with "[] [$]").
+      iApply contractsSound.
+      iIntros (_ _) "(%h1 & Hh1 & %Htrip)". clear Hverif.
+      destruct Htrip as [an Htrip].
+      iPoseProof (consume_sound _ _ Htrip with "Hh1")
+        as "[(Hpc & $ & Han) (%h2 & Hh2 & %HΦ)]".
+      iExists an. cbn. iFrame.
+      iExists h2. by iFrame.
+    Qed.
+
+    Lemma sound_exec_block_addr {instrs ainstr apc} Φ (h : SCHeap) :
+      cexec_block_addr instrs ainstr apc Φ h ->
+      interpret_scheap h ∗ lptsreg pc apc ∗ (∃ v, lptsreg nextpc v) ∗ ptsto_instrs ainstr instrs ⊢
+      (∀ an, lptsreg pc an ∗ (∃ v, lptsreg nextpc v) ∗ ptsto_instrs ainstr instrs ∗
+             (∃ h', interpret_scheap h' ∧ ⌜Φ an h'⌝) -∗ WP_loop) -∗ WP_loop.
+    Proof.
+      revert ainstr apc Φ h.
+      induction instrs as [|instr instrs]; cbn; intros ainstr apc Φ h;
+        cbv [bind assert_formula lift_purespec CPureSpec.assert_formula
+               CPureSpec.assert_pathcondition pure CPureSpec.pure].
+      - intros HΦ. iIntros "(Hpre & Hpc & Hnpc & _) Hk".
+        iApply "Hk"; iFrame; auto.
+      - intros [-> Hverif%sound_exec_instruction].
+        unfold semTripleOneInstrStep, semTriple in Hverif.
         iIntros "(Hh & Hpc & Hnpc & Hinstr & Hinstrs) Hk".
         iApply semWP_seq.
         iApply semWP_call_inline.
-        iApply (semWP_mono with "[Hh Hnpc Hpc Hinstr]").
-        { iApply ((sound_exec_instruction_any (fun an δ => (lptsreg pc an : iProp Σ) ∗ (∃ v, lptsreg nextpc v : iProp Σ) ∗ ptsto_instrs (bv.add apc bv_instrsize) (omap extract_AST instrs) -∗ (∀ an2 : Val ty_word, pc ↦ an2 ∗ (∃ v, nextpc ↦ v) ∗ ptsto_instrs (bv.add apc bv_instrsize) (omap extract_AST instrs) ∗ POST an2 [env] -∗ WP_loop) -∗ WP_loop)%I) with "[$]").
-          revert Hverif.
-          refine (mono_exec_instruction_any__c (h := h) _ _).
-          intros an h2.
-          unfold liftP; cbn.
-          iIntros (Hverif) "Hh2 (Hpc & Hnpc & Hinstrs) Hk".
-          iApply (IHinstrs (bv.add apc bv_instrsize)%Z an _ _ Hverif with "[$]").
-          iIntros (an2) "(Hpc & Hinstrs & HPOST)".
-          iApply "Hk"; now iFrame.
-        }
+        iApply (semWP_mono with "[-Hinstrs Hk] [Hinstrs Hk]").
+        iApply Hverif. iFrame. clear Hverif.
+        cbn.
         iIntros (_ _) "([%an (Hnpc & Hpc & Hk2)] & Hinstr)".
+        iDestruct "Hk2" as "(%h' & Hh' & %Hexec)".
+        specialize (IHinstrs _ _ _ _ Hexec). clear Hexec.
         iApply (semWP_call_inline loop).
-        iApply ("Hk2" with "[$Hpc Hnpc $Hinstrs]"); first by iExists _.
+        iApply (IHinstrs with "[$Hh' $Hpc Hnpc $Hinstrs]").
+        { now iExists an. }
         iIntros (an2) "(Hpc & Hnpc & Hinstrs & HPOST)".
         iApply ("Hk" with "[$]").
-      + iIntros (Hpost) "(Hh & Hpc & Hnpc & Hinstrs) Hk".
-        iApply ("Hk" with "[$Hpc $Hnpc $Hinstrs Hh]").
-        now iApply Hpost.
-      + iIntros (Hlemcall) "(Hh & Hpc & Hnpc & Hinstrs) Hk".
-        unfold bind, CStoreSpec.bind in Hlemcall; cbn.
-        unfold CStoreSpec.eval_exps in Hlemcall.
-        assert (CStoreSpec.call_lemma (LEnv lem) (evals es [env]) (fun _ => liftP (fun δ => lptsreg pc apc ∗ (∃ v : Val ty_xlenbits, lptsreg nextpc v) ∗ ptsto_instrs ainstr (omap extract_AST instrs) -∗
-                   (∀ an : Val ty_xlenbits, lptsreg pc an ∗ (∃ v : Val ty_xlenbits, lptsreg nextpc v) ∗ ptsto_instrs ainstr (omap extract_AST instrs) ∗ POST an [env] -∗ WP_loop) -∗ WP_loop)%I) [env] h) as Hcalllemma.
-        { revert Hlemcall.
-          apply call_lemma_monotonic.
-          intros _ δ h2.
-          destruct (env.view δ).
-          unfold liftP; cbn.
-          iIntros (Heb) "Hh2 (Hpc & Hnpc & Hinstrs) Hk".
-          iApply (IHinstrs _ _ _ _ Heb with "[$Hh2 $Hpc $Hnpc $Hinstrs]").
-          now iApply "Hk".
-        }
-        pose proof (Hlem := lemSem _ lem).
-        destruct (call_lemma_sound _ _ _ _ Hcalllemma).
-        cbn in *.
-        iPoseProof (H0 with "Hh") as "(%ι & _ & Hreq & Hk2)".
-        iApply ("Hk2" with "[Hreq] [$Hpc $Hnpc $Hinstrs] Hk").
-        now iApply Hlem.
-  Qed.
+    Qed.
 
-  Definition semTripleBlock `{sailGS Σ} (PRE : Val ty_word -> iProp Σ) (instrs : list AnnotInstr) (POST : Val ty_word -> Val ty_word -> iProp Σ) : iProp Σ :=
-    (∀ a,
-    (PRE a ∗ pc ↦ a ∗ (∃ v, nextpc ↦ v) ∗ ptsto_instrs a (omap extract_AST instrs)) -∗
-      (∀ an, pc ↦ an ∗ (∃ v, nextpc ↦ v) ∗ ptsto_instrs a (omap extract_AST instrs) ∗ POST a an -∗ WP_loop) -∗
-      WP_loop)%I.
-  Global Arguments semTripleBlock {Σ} {_} PRE%I instrs POST%I.
+    Lemma sound_cexec_triple_addr {Γ : LCtx} {pre post instrs} {ι : Valuation Γ} :
+      cexec_triple_addr pre instrs post (fun _ _ => True) []%list ->
+      ⊢ semTripleBlock (λ a : Val ty_word, asn.interpret pre (ι.[("a"::ty_xlenbits) ↦ a])) instrs
+          (λ a na : Val ty_word, asn.interpret post (ι.[("a"::ty_xlenbits) ↦ a].[("an"::ty_xlenbits) ↦ na])).
+    Proof.
+      cbv [cexec_triple_addr bind demonic_ctx demonic CPureSpec.demonic lift_purespec].
+      iIntros (Htrip a) "(Hpre & Hpc & Hnpc & Hinstrs) Hk".
+      rewrite CPureSpec.wp_demonic_ctx in Htrip.
+      specialize (Htrip ι a). apply produce_sound in Htrip.
+      iPoseProof (Htrip with "[$] Hpre") as "(%h2 & [Hh2 %Hexec])". clear Htrip.
+      apply sound_exec_block_addr in Hexec.
+      iApply (Hexec with "[$]"). clear Hexec.
+      iIntros (an2) "(Hpc & Hnpc & Hinstrs & (%h3 & [Hh3 %Hconsume]))".
+      apply consume_sound in Hconsume.
+      iPoseProof (Hconsume with "Hh3") as "[HPOST Hheap]".
+      iApply ("Hk" with "[$]").
+    Qed.
 
-  Lemma sound_exec_triple_addr__c `{sailGS Σ} {W : World} {pre post instrs} {ι : Valuation W} :
-    LemmaSem ->
-      (exec_triple_addr__c ι pre instrs post (λ _ _ _ , True) [env] []%list) ->
-    ⊢ semTripleBlock (λ a : Val ty_word, asn.interpret pre (ι.[("a"::ty_xlenbits) ↦ a])) instrs
-      (λ a na : Val ty_word, asn.interpret post (ι.[("a"::ty_xlenbits) ↦ a].[("an"::ty_xlenbits) ↦ na])).
-  Proof.
-    intros lemSem Hexec.
-    iIntros (a) "(Hpre & Hpc & Hnpc & Hinstrs) Hk".
-    specialize (Hexec a).
-    unfold bind, CStoreSpec.bind, produce in Hexec.
-    apply CHeapSpec.produce_sound in Hexec.
-    iPoseProof (Hexec with "[//] Hpre") as "(%h & Hh & %Hexec')". clear Hexec.
-    iApply ((sound_exec_block_addr (apc := a) h
-                  (fun an δ => asn.interpret post ι.["a"∷ty_word ↦ a].["an"∷ty_word ↦ an])%I)
-               with "[$Hh $Hpc $Hnpc $Hinstrs] Hk"); first easy.
-    revert Hexec'.
-    apply mono_exec_block_addr.
-    intros res h2 Hcons. cbn.
-    unfold liftP.
-    rewrite <-(bi.sep_True (asn.interpret _ _)).
-    eapply consume_sound.
-    revert Hcons.
-    apply CHeapSpec.mon_consume.
-    intros _ _ _ h3 _. auto.
-  Qed.
+    Lemma sound_cblock_verification_condition {Γ pre post instrs} :
+      cblock_verification_condition pre instrs post ->
+      forall ι : Valuation Γ,
+      ⊢ semTripleBlock (fun a => asn.interpret pre (ι.[("a"::ty_xlenbits) ↦ a]))
+          instrs
+          (fun a na => asn.interpret post (ι.[("a"::ty_xlenbits) ↦ a].[("an"::ty_xlenbits) ↦ na])).
+    Proof.
+      intros Hverif ι.
+      now apply sound_cexec_triple_addr.
+    Qed.
 
-  Lemma sound_VC__addr `{sailGS Σ} {Γ} {pre post instrs} :
-    LemmaSem ->
-    safeE (postprocess (BlockVerification3.VC__addr (Σ := Γ) pre instrs post)) ->
-    forall ι,
-    ⊢ semTripleBlock (fun a => asn.interpret pre (ι.[("a"::ty_xlenbits) ↦ a]))
-      instrs
-      (fun a na => asn.interpret post (ι.[("a"::ty_xlenbits) ↦ a].[("an"::ty_xlenbits) ↦ na])).
-  Proof.
-    intros lemSem Hverif ι.
-    apply (sound_exec_triple_addr__c (W := {| wctx := Γ ; wco := []%ctx |}) (pre := pre) (post := post) (instrs := instrs)); first easy.
-    eapply (fromEntails (refine_exec_triple_addr _ _ _ _) [env] I I _ (λ w1 _ _ _ _, SymProp.block)).
-    - done.
-    - eapply refine_lift; now cbn.
-    - now eapply logicalrelation.rlist_nil.
-    - rewrite inst_lift.
-      apply (fromBientails (w := wlctx Γ) LogicalSoundness.psafe_safe ι I).
+    Lemma sound_sblock_verification_condition {Γ pre post instrs} :
+      safeE (postprocess (sblock_verification_condition pre instrs post wnil)) ->
+      forall ι : Valuation Γ,
+      ⊢ semTripleBlock (fun a => asn.interpret pre (ι.[("a"::ty_xlenbits) ↦ a]))
+          instrs
+          (fun a na => asn.interpret post (ι.[("a"::ty_xlenbits) ↦ a].[("an"::ty_xlenbits) ↦ na])).
+    Proof.
+      intros Hverif ι.
+      apply sound_cexec_triple_addr.
       apply (safeE_safe env.nil), postprocess_sound in Hverif.
-      rewrite SymProp.safe_demonic_close in Hverif.
-      now apply Hverif.
-  Qed.
+      apply LogicalSoundness.psafe_safe in Hverif; [|done].
+      revert Hverif.
+      apply rexec_triple_addr.
+      - easy.
+      - easy.
+      - easy.
+      - constructor.
+    Qed.
 
-End BlockVerification3Sem.
+  End Soundness.
+
+End BlockVerificationDerived.
+
+Section AnnotatedBlockVerification.
+
+  Inductive AnnotInstr :=
+  | AnnotAST  (i : AST)
+  | AnnotDebugBreak
+  | AnnotLemmaInvocation {Δ} (l : 𝑳 Δ) (es : NamedEnv (Exp [ctx]) Δ)
+  .
+
+  Section Debug.
+
+    Import option.notations.
+
+    Record DebugBlockver (Σ : LCtx) : Type :=
+      MkDebugBlockver
+        { debug_blockver_pathcondition          : PathCondition Σ;
+          debug_blockver_heap                   : SHeap Σ;
+        }.
+    #[export] Instance SubstDebugBlockver : Subst DebugBlockver :=
+      fun Σ0 d Σ1 ζ01 =>
+        match d with
+        | MkDebugBlockver pc1 h => MkDebugBlockver (subst pc1 ζ01) (subst h ζ01)
+        end.
+
+    #[export] Instance SubstLawsDebugBlockver : SubstLaws DebugBlockver.
+    Proof.
+      constructor.
+      - intros ? []; cbn; now rewrite ?subst_sub_id.
+      - intros ? ? ? ? ? []; cbn; now rewrite ?subst_sub_comp.
+    Qed.
+
+    #[export] Instance OccursCheckDebugBlockver : OccursCheck DebugBlockver :=
+      fun Σ x xIn d =>
+        match d with
+        | MkDebugBlockver pc1 h =>
+            pc' <- occurs_check xIn pc1 ;;
+            h'  <- occurs_check xIn h ;;
+            Some (MkDebugBlockver pc' h')
+        end.
+
+  End Debug.
+
+  Import RiscvPmpBlockVerifSpec.
+
+  Section Symbolic.
+
+    Import ModalNotations.
+    Import SHeapSpec.
+    Import SHeapSpec.notations.
+
+    Fixpoint sexec_annotated_block_addr (b : list AnnotInstr) :
+      ⊢ STerm ty_xlenbits -> STerm ty_xlenbits -> SHeapSpec (STerm ty_xlenbits) :=
+      fun w0 ainstr apc =>
+        match b with
+        | nil       => pure apc
+        | cons instr b' =>
+            match instr with
+            | AnnotAST i =>
+                ⟨ θ1 ⟩ _    <- assert_formula
+                                 (fun _ => amsg.empty)
+                                 (formula_relop bop.eq ainstr apc) ;;
+                ⟨ θ2 ⟩ apc' <- sexec_instruction i (persist__term apc θ1) ;;
+                sexec_annotated_block_addr b'
+                  (term_binop bop.bvadd
+                     (persist__term ainstr (θ1 ∘ θ2))
+                     (term_val ty_word bv_instrsize))
+                  apc'
+            | AnnotDebugBreak =>
+                debug
+                  (fun (h0 : SHeap w0) =>
+                     amsg.mk
+                       {| debug_blockver_pathcondition := wco w0;
+                          debug_blockver_heap := h0
+                       |})
+                  (pure apc)
+            | AnnotLemmaInvocation l es =>
+                let args := seval_exps [env] es in
+                ⟨ θ1 ⟩ _ <- call_lemma (LEnv l) args ;;
+                sexec_annotated_block_addr b'
+                  (persist__term ainstr θ1)
+                  (persist__term apc θ1)
+            end
+        end.
+
+    Definition sexec_annotated_block_triple_addr {Σ : LCtx}
+      (req : Assertion (Σ ▻ ("a"::ty_xlenbits))) (b : list AnnotInstr)
+      (ens : Assertion (Σ ▻ ("a"::ty_xlenbits) ▻ ("an"::ty_xlenbits))) :
+      ⊢ SHeapSpec Unit :=
+      fun _ =>
+        ⟨ θ1 ⟩ lenv1 <- demonic_ctx id Σ ;;
+        ⟨ θ2 ⟩ a2 <- demonic (Some "a") _ ;;
+        let lenv2 := env.snoc (persist (A := Sub Σ) lenv1 θ2) _ a2 in
+        ⟨ θ3 ⟩ _ <- produce req lenv2 ;;
+        let a3 := persist__term a2 θ3 in
+        ⟨ θ4 ⟩ na <- sexec_annotated_block_addr b a3 a3 ;;
+        let lenv4 := persist lenv2 (θ3 ∘ θ4) in
+        consume ens lenv4.["an"∷ty_xlenbits ↦ na].
+
+    (* This is a VC for triples, for doubles we probably need to talk
+     about the continuation of a block. *)
+    Definition sannotated_block_verification_condition {Σ : LCtx}
+      (req : Assertion (Σ ▻ "a"∷ty_xlenbits)) (b : list AnnotInstr)
+      (ens : Assertion (Σ ▻ "a"∷ty_xlenbits ▻ "an"∷ty_xlenbits)) : ⊢ 𝕊 :=
+      (* SHeapSpec does not perform a leakcheck. We could include one here. *)
+      fun w => SHeapSpec.run (sexec_annotated_block_triple_addr req b ens (w := w)).
+
+  End Symbolic.
+
+  Section Shallow.
+
+    Import CHeapSpec CHeapSpec.notations.
+
+    Fixpoint cexec_annotated_block_addr (b : list AnnotInstr) :
+      Val ty_xlenbits -> Val ty_xlenbits -> CHeapSpec (Val ty_xlenbits) :=
+      fun ainstr apc =>
+        match b with
+        | nil       => pure apc
+        | cons instr b' =>
+            match instr with
+            | AnnotAST i =>
+                _ <- assert_formula (ainstr = apc) ;;
+                apc' <- cexec_instruction i apc ;;
+                cexec_annotated_block_addr b' (bv.add ainstr bv_instrsize) apc'
+            | AnnotDebugBreak => debug (pure apc)
+            | AnnotLemmaInvocation l es =>
+                let args := evals es [env] in
+                _ <- call_lemma (LEnv l) args ;;
+                cexec_annotated_block_addr b' ainstr apc
+            end
+        end.
+
+    Definition cexec_annotated_block_triple_addr {Σ}
+      (req : Assertion (Σ ▻ "a"∷ty_xlenbits)) (b : list AnnotInstr)
+      (ens : Assertion (Σ ▻ "a"∷ty_xlenbits ▻ "an"∷ty_xlenbits)) :
+      CHeapSpec unit :=
+      lenv <- demonic_ctx Σ ;;
+      a  <- demonic _ ;;
+      _  <- produce req lenv.["a"∷ty_xlenbits ↦ a]  ;;
+      na <- cexec_annotated_block_addr b a a ;;
+      consume ens lenv.["a"∷ty_xlenbits ↦ a].["an"∷ty_xlenbits ↦ na].
+
+    Definition cannotated_block_verification_condition {Σ : LCtx}
+      (req : Assertion (Σ ▻ "a"∷ty_xlenbits)) (b : list AnnotInstr)
+      (ens : Assertion (Σ ▻ "a"∷ty_xlenbits ▻ "an"∷ty_xlenbits)) : Prop :=
+      (* SHeapSpec does not perform a leakcheck. We could include one here. *)
+      CHeapSpec.run (cexec_annotated_block_triple_addr req b ens).
+
+    #[export] Instance mono_cexec_annotated_block_addr {instrs ainstr apc} :
+      Monotonic (MHeapSpec eq) (cexec_annotated_block_addr instrs ainstr apc).
+    Proof.
+      revert ainstr apc.
+      induction instrs; cbn; try typeclasses eauto.
+      destruct a; typeclasses eauto.
+    Qed.
+
+  End Shallow.
+
+  Section Relational.
+
+    Import RiscvPmpIrisInstanceWithContracts.StoreSpec.
+    Import logicalrelation logicalrelation.notations.
+    Import proofmode.
+    Import iris.proofmode.tactics.
+    Import RiscvPmpSignature.HeapSpec.
+
+    Lemma rexec_annotated_block_addr (b : list AnnotInstr) {w} :
+      ⊢ ℛ⟦RVal ty_xlenbits -> RVal ty_xlenbits -> RHeapSpec (RVal ty_xlenbits)⟧
+          (cexec_annotated_block_addr b)
+          (sexec_annotated_block_addr b (w := w)).
+    Proof.
+      iAssert (ℛ⟦□ᵣ (RVal ty_xlenbits -> RVal ty_xlenbits -> RHeapSpec (RVal ty_xlenbits))⟧
+                 (cexec_annotated_block_addr b)
+                 (fun w' θ => sexec_annotated_block_addr b (w := w'))) as "H".
+      { iInduction b as [|instr b] "IHb"; rsolve.
+        destruct instr; cbn; rsolve.
+        - iApply refine_assert_formula. rsolve.
+        - iApply "IHb"; rsolve.
+        - iApply refine_debug. rsolve.
+        - iApply refine_call_lemma. rsolve.
+          iApply refine_namedenv_nil.
+        - iApply "IHb"; rsolve.
+      }
+      now iApply (unconditionally_T with "H").
+    Qed.
+
+    Lemma rexec_annotated_block_triple_addr {Σ}
+      (req : Assertion (Σ ▻ "a"∷ty_xlenbits)) (b : list AnnotInstr)
+      (ens : Assertion (Σ ▻ "a"∷ty_xlenbits ▻ "an"∷ty_xlenbits)) {w} :
+      ⊢ ℛ⟦RHeapSpec RUnit⟧
+          (cexec_annotated_block_triple_addr req b ens)
+          (sexec_annotated_block_triple_addr req b ens (w := w)).
+    Proof.
+      unfold cexec_annotated_block_triple_addr, sexec_annotated_block_triple_addr.
+      rsolve.
+      iApply rexec_annotated_block_addr; rsolve.
+      rewrite !forgetting_trans.
+      iModIntro.
+      iModIntro.
+      rsolve.
+    Qed.
+
+    Lemma rannotated_block_verification_condition {Σ}
+      (req : Assertion (Σ ▻ "a"∷ty_xlenbits)) (b : list AnnotInstr)
+      (ens : Assertion (Σ ▻ "a"∷ty_xlenbits ▻ "an"∷ty_xlenbits)) {w} :
+      ⊢ ℛ⟦LogicalSoundness.RProp⟧
+          (cannotated_block_verification_condition req b ens)
+          (sannotated_block_verification_condition req b ens w).
+    Proof.
+      iApply HeapSpec.refine_run.
+      iApply rexec_annotated_block_triple_addr.
+    Qed.
+
+  End Relational.
+
+  Section Soundness.
+
+    Import iris.base_logic.lib.iprop iris.proofmode.tactics.
+    Import RiscvPmpIrisInstanceWithContracts.
+    Import ProgramLogic.
+    Import CHeapSpec.
+
+    Context {Σ} {GS : sailGS Σ}.
+
+    Definition extract_AST (i : AnnotInstr) : option AST :=
+      match i with
+      | AnnotAST a => Some a
+      | _ => None
+      end.
+
+    Lemma sound_exec_annotated_block_addr {instrs ainstr apc} (h : SCHeap) (POST : Val ty_xlenbits -> iProp Σ) :
+      LemmaSem ->
+      cexec_annotated_block_addr instrs ainstr apc (fun res h' => interpret_scheap h' ⊢ POST res) h ->
+      ⊢ ((interpret_scheap h ∗ lptsreg pc apc ∗ (∃ v, lptsreg nextpc v) ∗ ptsto_instrs ainstr (omap extract_AST instrs)) -∗
+         (∀ an, lptsreg pc an ∗ (∃ v, lptsreg nextpc v) ∗ ptsto_instrs ainstr (omap extract_AST instrs) ∗ POST an -∗ WP_loop) -∗
+         WP_loop)%I.
+    Proof.
+      intros lemSem.
+      revert ainstr apc h POST.
+      induction instrs as [|instr instrs]; cbn; intros ainstr apc h POST.
+      - iIntros (->) "(Hpre & Hpc & Hnpc & _) Hk".
+        iApply "Hk"; iFrame.
+      - cbv [bind assert_formula lift_purespec CPureSpec.assert_formula
+               CPureSpec.assert_pathcondition].
+        destruct instr as [instr| |Δ lem es].
+        + intros [-> Hverif]. cbn [extract_AST ptsto_instrs].
+          iIntros "(Hh & Hpc & Hnpc & Hinstr & Hinstrs) Hk".
+          iApply semWP_seq.
+          iApply semWP_call_inline.
+          iApply (semWP_mono with "[Hh Hnpc Hpc Hinstr]").
+          { iApply (sound_exec_instruction Hverif). iFrame. }
+          clear Hverif.
+          iIntros (_ _) "([%an (Hnpc & Hpc & (%h2 & Hh2 & %Hverif))] & Hinstr)".
+          iApply (semWP_call_inline loop).
+          specialize (IHinstrs _ _ _ _ Hverif).
+          iApply (IHinstrs with "[$Hh2 $Hpc Hnpc $Hinstrs]").
+          by iExists _.
+          iIntros (an2) "(Hpc & Hnpc & Hinstrs & HPOST)".
+          iApply ("Hk" with "[$]").
+        + cbv [debug pure lift_purespec CPureSpec.pure].
+          iIntros (->) "(Hh & Hpc & Hnpc & Hinstrs) Hk".
+          now iApply ("Hk" with "[$Hpc $Hnpc $Hinstrs Hh]").
+        + iIntros (Hlemcall) "(Hh & Hpc & Hnpc & Hinstrs) Hk".
+          assert (call_lemma (LEnv lem) (evals es [env])
+                    (fun _ h2 =>
+                       interpret_scheap h2 ⊢
+                       lptsreg pc apc ∗ (∃ v : Val ty_xlenbits, lptsreg nextpc v) ∗
+                       ptsto_instrs ainstr (omap extract_AST instrs) -∗
+                       (∀ an : Val ty_xlenbits,
+                          lptsreg pc an ∗ (∃ v : Val ty_xlenbits, lptsreg nextpc v) ∗
+                          ptsto_instrs ainstr (omap extract_AST instrs) ∗ POST an -∗ WP_loop)
+                       -∗ WP_loop) h) as Hcalllemma.
+          { revert Hlemcall. apply mon_call_lemma. intros _ _ _.
+            iIntros (h2 Heb) "Hh2 (Hpc & Hnpc & Hinstrs) Hk".
+            iApply (IHinstrs _ _ _ _ Heb with "[$Hh2 $Hpc $Hnpc $Hinstrs]").
+            now iApply "Hk".
+          }
+          clear Hlemcall.
+          pose proof (Hlem := lemSem _ lem).
+          apply call_lemma_sound in Hcalllemma.
+          destruct Hcalllemma.
+          cbn in *.
+          iPoseProof (H with "Hh") as "(%ι & _ & Hreq & Hk2)".
+          iApply ("Hk2" with "[Hreq] [$Hpc $Hnpc $Hinstrs] Hk").
+          now iApply Hlem.
+    Qed.
+
+    Definition semTripleAnnotatedBlock (PRE : Val ty_word -> iProp Σ)
+      (instrs : list AnnotInstr) (POST : Val ty_word -> Val ty_word -> iProp Σ) : iProp Σ :=
+      (∀ a,
+         (PRE a ∗ pc ↦ a ∗ (∃ v, nextpc ↦ v) ∗ ptsto_instrs a (omap extract_AST instrs)) -∗
+         (∀ an, pc ↦ an ∗ (∃ v, nextpc ↦ v) ∗ ptsto_instrs a (omap extract_AST instrs) ∗ POST a an -∗ WP_loop) -∗
+         WP_loop)%I.
+    Global Arguments semTripleAnnotatedBlock PRE%I instrs POST%I.
+
+    Lemma sound_cexec_annotated_block_triple_addr {Γ pre post instrs} :
+      LemmaSem ->
+      (cexec_annotated_block_triple_addr (Σ := Γ) pre instrs post (λ _ _ , True) []%list) ->
+      forall ι : Valuation Γ,
+      ⊢ semTripleAnnotatedBlock (λ a : Val ty_word, asn.interpret pre (ι.[("a"::ty_xlenbits) ↦ a])) instrs
+          (λ a na : Val ty_word, asn.interpret post (ι.[("a"::ty_xlenbits) ↦ a].[("an"::ty_xlenbits) ↦ na])).
+    Proof.
+      intros lemSem Hexec ι.
+      iIntros (a) "(Hpre & Hpc & Hnpc & Hinstrs) Hk".
+      hnf in Hexec.
+      rewrite CPureSpec.wp_demonic_ctx in Hexec.
+      specialize (Hexec ι a).
+      unfold bind in Hexec.
+      iPoseProof (produce_sound _ _ Hexec with "[//] [$Hpre]") as "(%h2 & Hh2 & %Hexec')".
+      clear Hexec.
+      iApply (sound_exec_annotated_block_addr (apc := a) h2 with "[$Hh2 $Hpc $Hnpc $Hinstrs]"); auto.
+      revert Hexec'.
+      apply mono_cexec_annotated_block_addr.
+      intros ? ? <- h3 Hcons.
+      iIntros "Hh3".
+      iPoseProof (consume_sound _ _ Hcons with "Hh3") as "[Hcons _]".
+      iFrame.
+    Qed.
+
+    Lemma sound_sannotated_block_verification_condition {Γ pre post instrs} :
+      LemmaSem ->
+      safeE (postprocess (sannotated_block_verification_condition (Σ := Γ)
+                            pre instrs post wnil)) ->
+      forall ι : Valuation Γ,
+      ⊢ semTripleAnnotatedBlock (fun a => asn.interpret pre (ι.[("a"::ty_xlenbits) ↦ a]))
+          instrs (fun a na => asn.interpret post (ι.[("a"::ty_xlenbits) ↦ a].[("an"::ty_xlenbits) ↦ na])).
+    Proof.
+      unfold sannotated_block_verification_condition, SHeapSpec.run.
+      intros lemSem Hverif ι.
+      apply sound_cexec_annotated_block_triple_addr; auto.
+      apply (safeE_safe env.nil), postprocess_sound in Hverif.
+      apply LogicalSoundness.psafe_safe in Hverif; [|done].
+      revert Hverif.
+      apply rexec_annotated_block_triple_addr.
+      - easy.
+      - easy.
+      - easy.
+      - constructor.
+    Qed.
+
+  End Soundness.
+
+End AnnotatedBlockVerification.
